Deficiency in Resource Space, use separation closed set instead of separation homorphic set

Phi_Semantics_Framework/Phi_Semantics_Framework.thy
@@ -128,7 +128,7 @@ unspecified_type RES
 unspecified_type RES_N
 type_synonym resource = \<open>RES_N \<Rightarrow> RES\<close>
 type_synonym rassn = \<open>resource set\<close>
-type_synonym 'T resource_entry = "(RES_N, RES, 'T) Resource_Space.kind"
+type_synonym 'T resource_entry = "(RES_N, RES, 'T, 'T sep_closed_set) Resource_Space.kind"
 
 setup \<open>Sign.mandatory_path "RES"\<close>
 
@@ -142,7 +142,7 @@ interpretation "resource_space" RES.DOMAIN .
 
 setup \<open>Sign.parent_path\<close>
 
-ML_file_debug \<open>resource_space_more.ML\<close>
+ML_file \<open>resource_space_more.ML\<close>
  
 ML \<open>Resource_Space.define_command \<^command_keyword>\<open>resource_space\<close> "extend resource semantics"\<close>
 
@@ -202,11 +202,11 @@ unspecified_type FIC_N
 
 type_synonym fiction = \<open>FIC_N \<Rightarrow> FIC\<close>
 type_synonym assn = \<open>fiction set\<close>
-type_synonym 'T fiction_entry = "(FIC_N, FIC, 'T) Resource_Space.kind"
+type_synonym 'T fiction_entry = "(FIC_N, FIC, 'T, unit) Resource_Space.kind"
 
 setup \<open>Sign.mandatory_path "FIC"\<close>
 
-consts DOMAIN :: \<open>FIC_N \<Rightarrow> FIC sep_closed_set\<close>
+consts DOMAIN :: \<open>FIC_N \<Rightarrow> FIC sep_homo_set\<close>
 
 debt_axiomatization sort: \<open>OFCLASS(FIC, sep_algebra_class)\<close>
 
